IsaSAT: more

Weidenbach_Book/Watched_Literals_Initialisation.thy
@@ -14,7 +14,7 @@ fun get_conflict_init :: \<open>'v twl_st_init \<Rightarrow> 'v cconflict\<close
   \<open>get_conflict_init ((_, _, _, D, _, _, _, _), _) = D\<close>
 
 fun literals_to_update_init :: \<open>'v twl_st_init \<Rightarrow> 'v clause\<close> where
-  \<open>literals_to_update_init ((_, _, _, _, _, _, _, Q), _) = Q\<close>
+  \<open>literals_to_update_init ((_, _, _, _, _, _, _, _, _, Q), _) = Q\<close>
 
 fun get_init_clauses_init :: \<open>'v twl_st_init \<Rightarrow> 'v twl_cls multiset\<close> where
   \<open>get_init_clauses_init ((_, N, _, _, _, _, _, _), _) = N\<close>
@@ -28,35 +28,41 @@ fun get_unit_init_clauses_init :: \<open>'v twl_st_init \<Rightarrow> 'v clauses
 fun get_unit_learned_clauses_init :: \<open>'v twl_st_init \<Rightarrow> 'v clauses\<close> where
   \<open>get_unit_learned_clauses_init ((_, _, _, _, _, UE, _, _), _) = UE\<close>
 
+fun get_subsumed_init_clauses_init :: \<open>'v twl_st_init \<Rightarrow> 'v clauses\<close> where
+  \<open>get_subsumed_init_clauses_init ((_, _, _, _, _, _, NS, US, _, _), _) = NS\<close>
+
+fun get_subsumed_learned_clauses_init :: \<open>'v twl_st_init \<Rightarrow> 'v clauses\<close> where
+  \<open>get_subsumed_learned_clauses_init ((_, _, _, _, _, _, NS, US, _, _), _) = US\<close>
+
 fun clauses_to_update_init :: \<open>'v twl_st_init \<Rightarrow> ('v literal \<times> 'v twl_cls) multiset\<close> where
-  \<open>clauses_to_update_init ((_, _, _, _, _, _, WS, _), _) = WS\<close>
+  \<open>clauses_to_update_init ((_, _, _, _, _, _, _, _, WS, _), _) = WS\<close>
 
 fun other_clauses_init :: \<open>'v twl_st_init \<Rightarrow> 'v clauses\<close> where
   \<open>other_clauses_init ((_, _, _, _, _, _, _), OC) = OC\<close>
 
 fun add_to_init_clauses :: \<open>'v clause_l \<Rightarrow> 'v twl_st_init \<Rightarrow> 'v twl_st_init\<close> where
-  \<open>add_to_init_clauses C ((M, N, U, D, NE, UE, WS, Q), OC) =
-      ((M, add_mset (twl_clause_of C) N, U, D, NE, UE, WS, Q), OC)\<close>
+  \<open>add_to_init_clauses C ((M, N, U, D, NE, UE, NS, US, WS, Q), OC) =
+      ((M, add_mset (twl_clause_of C) N, U, D, NE, UE, NS, US, WS, Q), OC)\<close>
 
 fun add_to_unit_init_clauses :: \<open>'v clause \<Rightarrow> 'v twl_st_init \<Rightarrow> 'v twl_st_init\<close> where
-  \<open>add_to_unit_init_clauses C ((M, N, U, D, NE, UE, WS, Q), OC) =
-      ((M, N, U, D, add_mset C NE, UE, WS, Q), OC)\<close>
+  \<open>add_to_unit_init_clauses C ((M, N, U, D, NE, UE, NS, US, WS, Q), OC) =
+      ((M, N, U, D, add_mset C NE, UE, NS, US, WS, Q), OC)\<close>
 
 fun set_conflict_init :: \<open>'v clause_l \<Rightarrow> 'v twl_st_init \<Rightarrow> 'v twl_st_init\<close> where
- \<open>set_conflict_init C ((M, N, U, _, NE, UE, WS, Q), OC) =
-       ((M, N, U, Some (mset C), add_mset (mset C) NE, UE, {#}, {#}), OC)\<close>
+ \<open>set_conflict_init C ((M, N, U, _, NE, UE, NS, US, WS, Q), OC) =
+       ((M, N, U, Some (mset C), add_mset (mset C) NE, UE, NS, US, {#}, {#}), OC)\<close>
 
 fun propagate_unit_init :: \<open>'v literal \<Rightarrow> 'v twl_st_init \<Rightarrow> 'v twl_st_init\<close> where
- \<open>propagate_unit_init L ((M, N, U, D, NE, UE, WS, Q), OC) =
-       ((Propagated L {#L#} # M, N, U, D, add_mset {#L#} NE, UE, WS, add_mset (-L) Q), OC)\<close>
+ \<open>propagate_unit_init L ((M, N, U, D, NE, UE, NS, US, WS, Q), OC) =
+       ((Propagated L {#L#} # M, N, U, D, add_mset {#L#} NE, UE, NS, US, WS, add_mset (-L) Q), OC)\<close>
 
 fun add_empty_conflict_init :: \<open>'v twl_st_init \<Rightarrow> 'v twl_st_init\<close> where
- \<open>add_empty_conflict_init ((M, N, U, D, NE, UE, WS, Q), OC) =
-       ((M, N, U, Some {#}, NE, UE, WS, {#}), add_mset {#} OC)\<close>
+ \<open>add_empty_conflict_init ((M, N, U, D, NE, UE, NS, US, WS, Q), OC) =
+       ((M, N, U, Some {#}, NE, UE, NS, US, WS, {#}), add_mset {#} OC)\<close>
 
 fun add_to_clauses_init :: \<open>'v clause_l \<Rightarrow> 'v twl_st_init \<Rightarrow> 'v twl_st_init\<close> where
-   \<open>add_to_clauses_init C ((M, N, U, D, NE, UE, WS, Q), OC) =
-        ((M, add_mset (twl_clause_of C) N, U, D, NE, UE, WS, Q), OC)\<close>
+   \<open>add_to_clauses_init C ((M, N, U, D, NE, UE, NS, US, WS, Q), OC) =
+        ((M, add_mset (twl_clause_of C) N, U, D, NE, UE, NS, US, WS, Q), OC)\<close>
 
 type_synonym 'v twl_st_l_init = \<open>'v twl_st_l \<times> 'v clauses\<close>
 
@@ -67,26 +73,32 @@ fun get_conflict_l_init :: \<open>'v twl_st_l_init \<Rightarrow> 'v cconflict\<c
   \<open>get_conflict_l_init ((_, _, D, _, _, _, _), _) = D\<close>
 
 fun get_unit_clauses_l_init :: \<open>'v twl_st_l_init \<Rightarrow> 'v clauses\<close> where
-  \<open>get_unit_clauses_l_init ((M, N, D, NE, UE, WS, Q), _) = NE + UE\<close>
+  \<open>get_unit_clauses_l_init ((M, N, D, NE, UE, NS, US, WS, Q), _) = NE + UE\<close>
 
 fun get_learned_unit_clauses_l_init :: \<open>'v twl_st_l_init \<Rightarrow> 'v clauses\<close> where
   \<open>get_learned_unit_clauses_l_init ((M, N, D, NE, UE, WS, Q), _) = UE\<close>
 
 fun get_clauses_l_init :: \<open>'v twl_st_l_init \<Rightarrow> 'v clauses_l\<close> where
-  \<open>get_clauses_l_init ((M, N, D, NE, UE, WS, Q), _) = N\<close>
+  \<open>get_clauses_l_init ((M, N, D, NE, UE, NS, US, WS, Q), _) = N\<close>
 
 fun literals_to_update_l_init :: \<open>'v twl_st_l_init \<Rightarrow> 'v clause\<close> where
-  \<open>literals_to_update_l_init ((_, _, _, _, _, _, Q), _) = Q\<close>
+  \<open>literals_to_update_l_init ((_, _, _, _, _, NS, US, _, Q), _) = Q\<close>
 
 fun clauses_to_update_l_init :: \<open>'v twl_st_l_init \<Rightarrow> 'v clauses_to_update_l\<close> where
-  \<open>clauses_to_update_l_init ((_, _, _, _, _, WS, _), _) = WS\<close>
+  \<open>clauses_to_update_l_init ((_, _, _, _, _, NS, US, WS, _), _) = WS\<close>
 
 fun other_clauses_l_init :: \<open>'v twl_st_l_init \<Rightarrow> 'v clauses\<close> where
   \<open>other_clauses_l_init ((_, _, _, _, _, _, _), OC) = OC\<close>
 
 fun state\<^sub>W_of_init :: "'v twl_st_init \<Rightarrow> 'v cdcl\<^sub>W_restart_mset" where
-"state\<^sub>W_of_init ((M, N, U, C, NE, UE, Q), OC) =
-  (M, clause `# N + NE + OC, clause `# U + UE, C)"
+"state\<^sub>W_of_init ((M, N, U, C, NE, UE, NS, US, Q), OC) =
+  (M, clause `# N + NE + NS + OC, clause `# U + UE + US, C)"
+
+fun get_subsumed_init_clauses_l_init :: \<open>'v twl_st_l_init \<Rightarrow> 'v clauses\<close> where
+  \<open>get_subsumed_init_clauses_l_init ((_, _, _, _, NS, US, _, _), _) = NS\<close>
+
+fun get_subsumed_learned_clauses_l_init :: \<open>'v twl_st_l_init \<Rightarrow> 'v clauses\<close> where
+  \<open>get_subsumed_learned_clauses_l_init ((M, N, D, NE, UE, NS, US, WS, Q), _) = US\<close>
 
 
 named_theorems twl_st_init \<open>Convertion for inital theorems\<close>
@@ -121,10 +133,10 @@ lemma [twl_st_init]:
   \<open>trail (state\<^sub>W_of_init T) = get_trail_init T\<close>
   \<open>get_trail (fst T) = get_trail_init (T)\<close>
   \<open>conflicting (state\<^sub>W_of_init T) = get_conflict_init T\<close>
-  \<open>init_clss (state\<^sub>W_of_init T) = clauses (get_init_clauses_init T) + get_unit_init_clauses_init T
-    + other_clauses_init T\<close>
+  \<open>init_clss (state\<^sub>W_of_init T) = clauses (get_init_clauses_init T) + get_unit_init_clauses_init T +
+    get_subsumed_init_clauses_init T + other_clauses_init T\<close>
   \<open>learned_clss (state\<^sub>W_of_init T) = clauses (get_learned_clauses_init T) +
-     get_unit_learned_clauses_init T\<close>
+     get_unit_learned_clauses_init T + get_subsumed_learned_clauses_init T\<close>
   \<open>conflicting (state\<^sub>W_of (fst T)) = conflicting (state\<^sub>W_of_init T)\<close>
   \<open>trail (state\<^sub>W_of (fst T)) = trail (state\<^sub>W_of_init T)\<close>
   \<open>clauses_to_update (fst T) = clauses_to_update_init T\<close>
@@ -133,11 +145,12 @@ lemma [twl_st_init]:
   by (cases T; auto simp: cdcl\<^sub>W_restart_mset_state; fail)+
 
 definition twl_st_l_init :: \<open>('v twl_st_l_init \<times> 'v twl_st_init) set\<close> where
-  \<open>twl_st_l_init = {(((M, N, C, NE, UE, WS, Q), OC), ((M', N', C', NE', UE', WS', Q'), OC')).
+  \<open>twl_st_l_init = {(((M, N, C, NE, UE, NS, US, WS, Q), OC),
+      ((M', N', C', NE', UE', NS', US', WS', Q'), OC')).
     (M , M') \<in> convert_lits_l N (NE+UE) \<and>
-    ((N', C', NE', UE', WS', Q'), OC') =
+    ((N', C', NE', UE', NS', US', WS', Q'), OC') =
       ((twl_clause_of `# init_clss_lf N, twl_clause_of `# learned_clss_lf N,
-         C, NE, UE, {#}, Q), OC)}\<close>
+         C, NE, UE, NS, US, {#}, Q), OC)}\<close>
 
 lemma twl_st_l_init_alt_def:
   \<open>(S, T) \<in> twl_st_l_init \<longleftrightarrow>
@@ -170,7 +183,8 @@ definition twl_struct_invs_init :: \<open>'v twl_st_init \<Rightarrow> bool\<clo
     (get_conflict_init S \<noteq> None \<longrightarrow> clauses_to_update_init S = {#} \<and> literals_to_update_init S = {#}) \<and>
     entailed_clss_inv (fst S) \<and>
     clauses_to_update_inv (fst S) \<and>
-    past_invs (fst S))
+    past_invs (fst S)) \<and>
+    subsumed_clauses_inv (fst S)
   \<close>
 
 lemma state\<^sub>W_of_state\<^sub>W_of_init:
@@ -202,7 +216,8 @@ proof -
     confl: \<open>get_conflict S \<noteq> None \<longrightarrow> clauses_to_update S = {#} \<and> literals_to_update S = {#}\<close> and
     unit: \<open>entailed_clss_inv S\<close> and
     to_upd: \<open>clauses_to_update_inv S\<close> and
-    past: \<open>past_invs S\<close>
+    past: \<open>past_invs S\<close> and
+    subs: \<open>subsumed_clauses_inv S\<close>
     using assms unfolding twl_struct_invs_init_def fst_conv
     by (auto simp add: twl_st_init)
 
@@ -230,40 +245,41 @@ proof -
     subgoal by (rule unit)
     subgoal by (rule to_upd)
     subgoal by (rule past)
+    subgoal by (rule subs)
     done
 qed
 
 fun add_empty_conflict_init_l :: \<open>'v twl_st_l_init \<Rightarrow> 'v twl_st_l_init\<close> where
   add_empty_conflict_init_l_def[simp del]:
-   \<open>add_empty_conflict_init_l ((M, N, D, NE, UE, WS, Q), OC) =
-       ((M, N, Some {#}, NE, UE, WS, {#}), add_mset {#} OC)\<close>
+   \<open>add_empty_conflict_init_l ((M, N, D, NE, UE, NS, US, WS, Q), OC) =
+       ((M, N, Some {#}, NE, UE, NS, US, WS, {#}), add_mset {#} OC)\<close>
 
 
 fun propagate_unit_init_l :: \<open>'v literal \<Rightarrow> 'v twl_st_l_init \<Rightarrow> ('v twl_st_l_init) nres\<close> where
   propagate_unit_init_l_def[simp del]:
-   \<open>propagate_unit_init_l L ((M, N, D, NE, UE, WS, Q), OC) = do {
+   \<open>propagate_unit_init_l L ((M, N, D, NE, UE, NS, US, WS, Q), OC) = do {
        M \<leftarrow> cons_trail_propagate_l L 0 M;
-       RETURN ((M, N, D, add_mset {#L#} NE, UE, WS, add_mset (-L) Q), OC)
+       RETURN ((M, N, D, add_mset {#L#} NE, UE, NS, US, WS, add_mset (-L) Q), OC)
      }\<close>
 
 
 fun already_propagated_unit_init_l :: \<open>'v clause \<Rightarrow> 'v twl_st_l_init \<Rightarrow> 'v twl_st_l_init\<close> where
   already_propagated_unit_init_l_def[simp del]:
-   \<open>already_propagated_unit_init_l C ((M, N, D, NE, UE, WS, Q), OC) =
-       ((M, N, D, add_mset C NE, UE, WS, Q), OC)\<close>
+   \<open>already_propagated_unit_init_l C ((M, N, D, NE, UE, NS, US, WS, Q), OC) =
+       ((M, N, D, add_mset C NE, UE, NS, US, WS, Q), OC)\<close>
 
 
 fun set_conflict_init_l :: \<open>'v clause_l \<Rightarrow> 'v twl_st_l_init \<Rightarrow> 'v twl_st_l_init\<close> where
   set_conflict_init_l_def[simp del]:
-   \<open>set_conflict_init_l C ((M, N, _, NE, UE, WS, Q), OC) =
-       ((M, N, Some (mset C), add_mset (mset C) NE, UE, {#}, {#}), OC)\<close>
+   \<open>set_conflict_init_l C ((M, N, _, NE, UE, NS, US, WS, Q), OC) =
+       ((M, N, Some (mset C), add_mset (mset C) NE, UE, NS, US, {#}, {#}), OC)\<close>
 
 
 fun add_to_clauses_init_l :: \<open>'v clause_l \<Rightarrow> 'v twl_st_l_init \<Rightarrow> 'v twl_st_l_init nres\<close> where
   add_to_clauses_init_l_def[simp del]:
-   \<open>add_to_clauses_init_l C ((M, N, _, NE, UE, WS, Q), OC) = do {
+   \<open>add_to_clauses_init_l C ((M, N, _, NE, UE, NS, US, WS, Q), OC) = do {
         i \<leftarrow> get_fresh_index N;
-        RETURN ((M, fmupd i (C, True) N, None, NE, UE, WS, Q), OC)
+        RETURN ((M, fmupd i (C, True) N, None, NE, UE, NS, US, WS, Q), OC)
     }\<close>
 
 fun add_to_other_init where
@@ -344,13 +360,14 @@ lemma twl_struct_invs_init_add_to_other_init:
     \<open>twl_struct_invs_init (add_to_other_init a T)\<close>
       (is ?twl_struct_invs_init)
 proof -
-  obtain M N U D NE UE Q OC WS where
-    T: \<open>T = ((M, N, U, D, NE, UE, WS, Q), OC)\<close>
+  obtain M N U D NE UE Q OC WS NS US  where
+    T: \<open>T = ((M, N, U, D, NE, UE, NS, US, WS, Q), OC)\<close>
     by (cases T) auto
-  have \<open>cdcl\<^sub>W_restart_mset.cdcl\<^sub>W_all_struct_inv (M, clauses N + NE + OC, clauses U + UE, D)\<close>
+  have \<open>cdcl\<^sub>W_restart_mset.cdcl\<^sub>W_all_struct_inv (M, clauses N + NE + NS + OC, clauses U + UE + US, D)\<close>
     using invs unfolding T twl_struct_invs_init_def by auto
   then have [simp]:
-   \<open>cdcl\<^sub>W_restart_mset.cdcl\<^sub>W_all_struct_inv (M, add_mset (mset a) (clauses N + NE + OC), clauses U + UE, D)\<close>
+   \<open>cdcl\<^sub>W_restart_mset.cdcl\<^sub>W_all_struct_inv (M, add_mset (mset a) (clauses N + NE + NS + OC),
+      clauses U + UE + US, D)\<close>
     using dist
     by (auto simp: cdcl\<^sub>W_restart_mset.cdcl\<^sub>W_all_struct_inv_def
        cdcl\<^sub>W_restart_mset.no_strange_atm_def cdcl\<^sub>W_restart_mset_state
@@ -359,11 +376,11 @@ proof -
        clauses_def cdcl\<^sub>W_restart_mset.cdcl\<^sub>W_learned_clause_alt_def
        cdcl\<^sub>W_restart_mset.reasons_in_clauses_def)
 
-  have \<open>cdcl\<^sub>W_restart_mset.no_smaller_propa (M, clauses N + NE + OC, clauses U + UE, D)\<close>
+  have \<open>cdcl\<^sub>W_restart_mset.no_smaller_propa (M, clauses N + NE + NS + OC, clauses U + UE + US, D)\<close>
     using invs unfolding T twl_struct_invs_init_def by auto
   then have [simp]:
-     \<open>cdcl\<^sub>W_restart_mset.no_smaller_propa (M, add_mset (mset a) (clauses N + NE + OC),
-        clauses U + UE, D)\<close>
+     \<open>cdcl\<^sub>W_restart_mset.no_smaller_propa (M, add_mset (mset a) (clauses N + NE + NS + OC),
+        clauses U + UE + US, D)\<close>
     using lev
     by (auto simp: cdcl\<^sub>W_restart_mset.no_smaller_propa_def cdcl\<^sub>W_restart_mset_state
         clauses_def T count_decided_0_iff)
@@ -386,8 +403,8 @@ lemma invariants_init_state:
     \<open>clauses_to_update_inv (fst T)\<close> and \<open>past_invs (fst T)\<close> and \<open>distinct_queued (fst T)\<close> and
     \<open>valid_enqueued (fst T)\<close> and \<open>twl_st_exception_inv (fst T)\<close> and \<open>no_duplicate_queued (fst T)\<close>
 proof -
-  obtain M N U NE UE OC D where
-    T: \<open>T = ((M, N, U, D, NE, UE, {#}, uminus `# lit_of `# mset M), OC)\<close>
+  obtain M N U NE UE OC D NS US where
+    T: \<open>T = ((M, N, U, D, NE, UE, NS, US, {#}, uminus `# lit_of `# mset M), OC)\<close>
     using MQ WS by (cases T) auto
   let ?Q = \<open>uminus `# lit_of `# mset M\<close>
 
@@ -472,6 +489,7 @@ lemma twl_struct_invs_init_init_state:
     \<open>cdcl\<^sub>W_restart_mset.no_smaller_propa (state\<^sub>W_of_init T)\<close> and
     \<open>entailed_clss_inv (fst T)\<close> and
     \<open>get_conflict_init T \<noteq> None \<longrightarrow> clauses_to_update_init T = {#} \<and> literals_to_update_init T = {#}\<close>
+    \<open>subsumed_clauses_inv (fst T)\<close>
   shows \<open>twl_struct_invs_init T\<close>
 proof -
   have n_d: \<open>no_dup (get_trail_init T)\<close>
@@ -493,40 +511,41 @@ lemma twl_struct_invs_init_add_to_unit_init_clauses:
     \<open>twl_struct_invs_init (add_to_unit_init_clauses (mset a) T)\<close>
       (is ?all_struct)
 proof -
-  obtain M N U D NE UE Q OC WS where
-    T: \<open>T = ((M, N, U, D, NE, UE, WS, Q), OC)\<close>
+  obtain M N U D NE UE Q NS US OC WS where
+    T: \<open>T = ((M, N, U, D, NE, UE, NS, US, WS, Q), OC)\<close>
     by (cases T) auto
-  have \<open>cdcl\<^sub>W_restart_mset.cdcl\<^sub>W_all_struct_inv (M, clauses N + NE + OC, clauses U + UE, D)\<close>
+  have \<open>cdcl\<^sub>W_restart_mset.cdcl\<^sub>W_all_struct_inv (M, clauses N + NE + NS + OC, clauses U + UE + US, D)\<close>
     using invs unfolding T twl_struct_invs_init_def by auto
   then have [simp]:
-   \<open>cdcl\<^sub>W_restart_mset.cdcl\<^sub>W_all_struct_inv (M, add_mset (mset a) (clauses N + NE + OC), clauses U + UE, D)\<close>
+   \<open>cdcl\<^sub>W_restart_mset.cdcl\<^sub>W_all_struct_inv (M, add_mset (mset a) (clauses N + NE + NS + OC),
+      clauses U + UE + US, D)\<close>
     using twl_struct_invs_init_add_to_other_init[OF dist lev invs]
     unfolding T twl_struct_invs_init_def
     by simp
 
-  have \<open>cdcl\<^sub>W_restart_mset.no_smaller_propa (M, clauses N + NE + OC, clauses U + UE, D)\<close>
+  have \<open>cdcl\<^sub>W_restart_mset.no_smaller_propa (M, clauses N + NE + NS + OC, clauses U + UE + US, D)\<close>
     using invs unfolding T twl_struct_invs_init_def by auto
   then have [simp]:
-     \<open>cdcl\<^sub>W_restart_mset.no_smaller_propa (M, add_mset (mset a) (clauses N + NE + OC),
-        clauses U + UE, D)\<close>
+     \<open>cdcl\<^sub>W_restart_mset.no_smaller_propa (M, add_mset (mset a) (clauses N + NE + NS + OC),
+        clauses U + UE + US, D)\<close>
     using lev
     by (auto simp: cdcl\<^sub>W_restart_mset.no_smaller_propa_def cdcl\<^sub>W_restart_mset_state
         clauses_def T count_decided_0_iff)
-  have [simp]: \<open>confl_cands_enqueued (M, N, U, D, add_mset (mset a) NE, UE, WS, Q) \<longleftrightarrow>
-     confl_cands_enqueued (M, N, U, D, NE, UE, WS, Q)\<close>
-    \<open>propa_cands_enqueued (M, N, U, D, add_mset (mset a) NE, UE, WS, Q) \<longleftrightarrow>
-      propa_cands_enqueued (M, N, U, D, NE, UE, WS, Q)\<close>
-    \<open>twl_st_inv (M, N, U, D, add_mset (mset a) NE, UE, WS, Q) \<longleftrightarrow>
-        twl_st_inv (M, N, U, D, NE, UE, WS, Q)\<close>
-    \<open>\<And>x.  twl_exception_inv (M, N, U, D, add_mset (mset a) NE, UE, WS, Q) x \<longleftrightarrow>
-          twl_exception_inv (M, N, U, D, NE, UE, WS, Q) x\<close>
-    \<open>clauses_to_update_inv (M, N, U, D, add_mset (mset a) NE, UE, WS, Q) \<longleftrightarrow>
-       clauses_to_update_inv (M, N, U, D, NE, UE, WS, Q)\<close>
-    \<open>past_invs (M, N, U, D, add_mset (mset a) NE, UE, WS, Q) \<longleftrightarrow>
-        past_invs (M, N, U, D, NE, UE, WS, Q)\<close>
+  have [simp]: \<open>confl_cands_enqueued (M, N, U, D, add_mset (mset a) NE, UE, NS, US, WS, Q) \<longleftrightarrow>
+     confl_cands_enqueued (M, N, U, D, NE, UE, NS, US, WS, Q)\<close>
+    \<open>propa_cands_enqueued (M, N, U, D, add_mset (mset a) NE, UE, NS, US, WS, Q) \<longleftrightarrow>
+      propa_cands_enqueued (M, N, U, D, NE, UE, NS, US, WS, Q)\<close>
+    \<open>twl_st_inv (M, N, U, D, add_mset (mset a) NE, UE, NS, US, WS, Q) \<longleftrightarrow>
+        twl_st_inv (M, N, U, D, NE, UE, NS, US, WS, Q)\<close>
+    \<open>\<And>x.  twl_exception_inv (M, N, U, D, add_mset (mset a) NE, UE, NS, US, WS, Q) x \<longleftrightarrow>
+          twl_exception_inv (M, N, U, D, NE, UE, NS, US, WS, Q) x\<close>
+    \<open>clauses_to_update_inv (M, N, U, D, add_mset (mset a) NE, UE, NS, US, WS, Q) \<longleftrightarrow>
+       clauses_to_update_inv (M, N, U, D, NE, UE, NS, US, WS, Q)\<close>
+    \<open>past_invs (M, N, U, D, add_mset (mset a) NE, UE, NS, US, WS, Q) \<longleftrightarrow>
+        past_invs (M, N, U, D, NE, UE, NS, US, WS, Q)\<close>
     by (cases D; auto simp: twl_st_inv.simps twl_exception_inv.simps past_invs.simps; fail)+
-  have [simp]: \<open>entailed_clss_inv (M, N, U, D, add_mset (mset a) NE, UE, WS, Q) \<longleftrightarrow>
-     entailed_clss_inv (M, N, U, D, NE, UE, WS, Q)\<close>
+  have [simp]: \<open>entailed_clss_inv (M, N, U, D, add_mset (mset a) NE, UE, NS, US, WS, Q) \<longleftrightarrow>
+     entailed_clss_inv (M, N, U, D, NE, UE, NS, US, WS, Q)\<close>
     using ex count_decided_ge_get_level[of M] lev by (cases D) (auto simp: T)
   show ?all_struct
     using invs ex
@@ -546,14 +565,14 @@ lemma twl_struct_invs_init_set_conflict_init:
     \<open>twl_struct_invs_init (set_conflict_init C T)\<close>
       (is ?all_struct)
 proof -
-  obtain M N U D NE UE Q OC WS where
-    T: \<open>T = ((M, N, U, D, NE, UE, WS, Q), OC)\<close>
+  obtain M N U D NE UE Q OC WS NS US where
+    T: \<open>T = ((M, N, U, D, NE, UE, NS, US, WS, Q), OC)\<close>
     by (cases T) auto
-  have \<open>cdcl\<^sub>W_restart_mset.cdcl\<^sub>W_all_struct_inv (M, clauses N + NE + OC, clauses U + UE, D)\<close>
+  have \<open>cdcl\<^sub>W_restart_mset.cdcl\<^sub>W_all_struct_inv (M, clauses N + NE + NS + OC, clauses U + UE + US, D)\<close>
     using invs unfolding T twl_struct_invs_init_def by auto
   then have [simp]:
-   \<open>cdcl\<^sub>W_restart_mset.cdcl\<^sub>W_all_struct_inv (M, add_mset (mset C) (clauses N + NE + OC),
-        clauses U + UE, Some (mset C))\<close>
+   \<open>cdcl\<^sub>W_restart_mset.cdcl\<^sub>W_all_struct_inv (M, add_mset (mset C) (clauses N + NE + NS + OC),
+        clauses U + UE + US, Some (mset C))\<close>
     using dist ex
     unfolding T twl_struct_invs_init_def
     by (auto 5 5 simp: cdcl\<^sub>W_restart_mset.cdcl\<^sub>W_all_struct_inv_def
@@ -563,24 +582,24 @@ proof -
        clauses_def cdcl\<^sub>W_restart_mset.cdcl\<^sub>W_learned_clause_alt_def
        true_annots_true_cls_def_iff_negation_in_model)
 
-  have \<open>cdcl\<^sub>W_restart_mset.no_smaller_propa (M, clauses N + NE + OC, clauses U + UE, D)\<close>
+  have \<open>cdcl\<^sub>W_restart_mset.no_smaller_propa (M, clauses N + NE + NS + OC, clauses U + UE + US, D)\<close>
     using invs unfolding T twl_struct_invs_init_def by auto
   then have [simp]:
-     \<open>cdcl\<^sub>W_restart_mset.no_smaller_propa (M, add_mset (mset C) (clauses N + NE + OC),
-        clauses U + UE, Some (mset C))\<close>
+     \<open>cdcl\<^sub>W_restart_mset.no_smaller_propa (M, add_mset (mset C) (clauses N + NE + NS + OC),
+        clauses U + UE + US, Some (mset C))\<close>
     using lev
     by (auto simp: cdcl\<^sub>W_restart_mset.no_smaller_propa_def cdcl\<^sub>W_restart_mset_state
         clauses_def T count_decided_0_iff)
-  let ?T = \<open>(M, N, U, Some (mset C), add_mset (mset C) NE, UE, {#}, {#})\<close>
+  let ?T = \<open>(M, N, U, Some (mset C), add_mset (mset C) NE, UE, NS, US, {#}, {#})\<close>
 
   have [simp]: \<open>confl_cands_enqueued ?T\<close>
     \<open>propa_cands_enqueued ?T\<close>
-    \<open>twl_st_inv (M, N, U, D, NE, UE, WS, Q) \<Longrightarrow> twl_st_inv ?T\<close>
-    \<open>\<And>x.  twl_exception_inv (M, N, U, D, NE, UE, WS, Q) x \<Longrightarrow> twl_exception_inv ?T x\<close>
-    \<open>clauses_to_update_inv (M, N, U, D, NE, UE, WS, Q) \<Longrightarrow> clauses_to_update_inv ?T\<close>
-    \<open>past_invs (M, N, U, D, NE, UE, WS, Q) \<Longrightarrow> past_invs ?T\<close>
+    \<open>twl_st_inv (M, N, U, D, NE, UE, NS, US, WS, Q) \<Longrightarrow> twl_st_inv ?T\<close>
+    \<open>\<And>x.  twl_exception_inv (M, N, U, D, NE, UE, NS, US, WS, Q) x \<Longrightarrow> twl_exception_inv ?T x\<close>
+    \<open>clauses_to_update_inv (M, N, U, D, NE, UE, NS, US, WS, Q) \<Longrightarrow> clauses_to_update_inv ?T\<close>
+    \<open>past_invs (M, N, U, D, NE, UE, NS, US, WS, Q) \<Longrightarrow> past_invs ?T\<close>
     by (auto simp: twl_st_inv.simps twl_exception_inv.simps past_invs.simps; fail)+
-  have [simp]: \<open>entailed_clss_inv (M, N, U, D, NE, UE, WS, Q) \<Longrightarrow> entailed_clss_inv ?T\<close>
+  have [simp]: \<open>entailed_clss_inv (M, N, U, D, NE, UE, NS, US, WS, Q) \<Longrightarrow> entailed_clss_inv ?T\<close>
     using ex count_decided_ge_get_level[of M] lev nempty by (auto simp: T)
   show ?all_struct
     using invs ex
@@ -601,8 +620,8 @@ lemma twl_struct_invs_init_propagate_unit_init:
     \<open>twl_struct_invs_init (propagate_unit_init L T)\<close>
       (is ?all_struct)
 proof -
-  obtain M N U NE UE OC WS where
-    T: \<open>T = ((M, N, U, None, NE, UE, WS, uminus `# lit_of `# mset M), OC)\<close>
+  obtain M N U NE UE OC WS NS US where
+    T: \<open>T = ((M, N, U, None, NE, UE, NS, US, WS, uminus `# lit_of `# mset M), OC)\<close>
     using confl MQ by (cases T) auto
   let ?Q = \<open>uminus `# lit_of `# mset M\<close>
   have [iff]: \<open>- L \<in> lits_of_l M \<longleftrightarrow> False\<close>
@@ -614,13 +633,13 @@ proof -
      (a \<noteq> [] \<and> hd a = Propagated L mark \<and> tl a @ Propagated L' mark' # b = M)\<close>
     for a mark mark' L' b
     using undef by (cases a) (auto simp: T atm_of_eq_atm_of)
-  have \<open>cdcl\<^sub>W_restart_mset.cdcl\<^sub>W_all_struct_inv (M, clauses N + NE + OC, clauses U + UE,  None)\<close> and
-    excep: \<open>twl_st_exception_inv (M, N, U, None, NE, UE, WS, ?Q)\<close> and
-    st_inv: \<open>twl_st_inv (M, N, U, None, NE, UE, WS, ?Q)\<close>
+  have \<open>cdcl\<^sub>W_restart_mset.cdcl\<^sub>W_all_struct_inv (M, clauses N + NE + NS + OC, clauses U + UE + US,  None)\<close> and
+    excep: \<open>twl_st_exception_inv (M, N, U, None, NE, UE, NS, US, WS, ?Q)\<close> and
+    st_inv: \<open>twl_st_inv (M, N, U, None, NE, UE, NS, US, WS, ?Q)\<close>
     using invs confl unfolding T twl_struct_invs_init_def by auto
   then have [simp]:
-   \<open>cdcl\<^sub>W_restart_mset.cdcl\<^sub>W_all_struct_inv (M, add_mset {#L#} (clauses N + NE + OC),
-     clauses U + UE, None)\<close> and
+   \<open>cdcl\<^sub>W_restart_mset.cdcl\<^sub>W_all_struct_inv (M, add_mset {#L#} (clauses N + NE + NS + OC),
+     clauses U + UE + US, None)\<close> and
    n_d: \<open>no_dup M\<close>
     by (auto simp: cdcl\<^sub>W_restart_mset.cdcl\<^sub>W_all_struct_inv_def
        cdcl\<^sub>W_restart_mset.no_strange_atm_def cdcl\<^sub>W_restart_mset_state
@@ -630,7 +649,7 @@ proof -
        cdcl\<^sub>W_restart_mset.reasons_in_clauses_def)
   then have [simp]:
    \<open>cdcl\<^sub>W_restart_mset.cdcl\<^sub>W_all_struct_inv (Propagated L {#L#} # M,
-        add_mset {#L#} (clauses N + NE + OC), clauses U + UE, None)\<close>
+        add_mset {#L#} (clauses N + NE + NS + OC), clauses U + UE + US, None)\<close>
     using undef by (auto simp: cdcl\<^sub>W_restart_mset.cdcl\<^sub>W_all_struct_inv_def T H
         cdcl\<^sub>W_restart_mset.no_strange_atm_def cdcl\<^sub>W_restart_mset_state
         cdcl\<^sub>W_restart_mset.cdcl\<^sub>W_M_level_inv_def cdcl\<^sub>W_restart_mset.cdcl\<^sub>W_conflicting_def
@@ -639,31 +658,32 @@ proof -
         consistent_interp_insert_iff)
   have [iff]: \<open>Propagated L {#L#} # M = M' @ Decided K # Ma \<longleftrightarrow> False\<close> for M' K Ma
     using lev by (cases M') (auto simp: count_decided_0_iff T)
-  have \<open>cdcl\<^sub>W_restart_mset.no_smaller_propa (M, clauses N + NE + OC, clauses U + UE, None)\<close>
+  have \<open>cdcl\<^sub>W_restart_mset.no_smaller_propa (M, clauses N + NE + NS + OC, clauses U + UE + US, None)\<close>
     using invs confl unfolding T twl_struct_invs_init_def by auto
   then have [simp]:
-     \<open>cdcl\<^sub>W_restart_mset.no_smaller_propa (Propagated L {#L#} # M, add_mset {#L#} (clauses N + NE + OC),
-        clauses U + UE,  None)\<close>
+     \<open>cdcl\<^sub>W_restart_mset.no_smaller_propa (Propagated L {#L#} # M, add_mset {#L#} (clauses N + NE + NS + OC),
+        clauses U + UE + US,  None)\<close>
     using lev
     by (auto simp: cdcl\<^sub>W_restart_mset.no_smaller_propa_def cdcl\<^sub>W_restart_mset_state
         clauses_def T count_decided_0_iff)
 
-  have \<open>cdcl\<^sub>W_restart_mset.no_smaller_propa (M, clauses N + NE + OC, clauses U + UE, None)\<close>
+  have \<open>cdcl\<^sub>W_restart_mset.no_smaller_propa (M, clauses N + NE + NS + OC, clauses U + UE + US, None)\<close>
     using invs confl unfolding T twl_struct_invs_init_def by auto
   then have [simp]:
-     \<open>cdcl\<^sub>W_restart_mset.no_smaller_propa (Propagated L {#L#} # M, add_mset {#L#} (clauses N + NE + OC),
-        clauses U + UE, None)\<close>
+     \<open>cdcl\<^sub>W_restart_mset.no_smaller_propa (Propagated L {#L#} # M, add_mset {#L#} (clauses N + NE + NS + OC),
+        clauses U + UE + US, None)\<close>
     using lev
     by (auto simp: cdcl\<^sub>W_restart_mset.no_smaller_propa_def cdcl\<^sub>W_restart_mset_state
         clauses_def T count_decided_0_iff)
-  let ?S = \<open>(M, N, U, None, NE, UE, WS, ?Q)\<close>
-  let ?T = \<open>(Propagated L {#L#} # M, N, U, None, add_mset {#L#} NE, UE, WS, add_mset (-L) ?Q)\<close>
+  let ?S = \<open>(M, N, U, None, NE, UE, NS, US, WS, ?Q)\<close>
+  let ?T = \<open>(Propagated L {#L#} # M, N, U, None, add_mset {#L#} NE, UE, NS, US, WS, add_mset (-L) ?Q)\<close>
 
   have struct: \<open>struct_wf_twl_cls C\<close> if \<open>C \<in># N + U\<close> for C
     using st_inv that by (simp add: twl_st_inv.simps)
-  have \<open>entailed_clss_inv (fst T)\<close>
-    using invs unfolding T twl_struct_invs_init_def fst_conv by fast
-  then have ent: \<open>entailed_clss_inv (fst (propagate_unit_init L T))\<close>
+  have \<open>entailed_clss_inv (fst T)\<close> \<open>subsumed_clauses_inv (fst T)\<close>
+    using invs unfolding T twl_struct_invs_init_def fst_conv by fast+
+  then have ent: \<open>entailed_clss_inv (fst (propagate_unit_init L T))\<close> and
+    subs: \<open>subsumed_clauses_inv (fst (propagate_unit_init L T))\<close>
     using lev by (auto simp: T get_level_cons_if)
   show \<open>twl_struct_invs_init (propagate_unit_init L T)\<close>
     apply (rule twl_struct_invs_init_init_state)
@@ -675,6 +695,7 @@ proof -
     subgoal by (auto simp: T)
     subgoal by (rule ent)
     subgoal by (auto simp: T)
+    subgoal by (rule subs)
     done
 qed
 
@@ -690,6 +711,10 @@ lemma [twl_st_l_init]:
   \<open>get_unit_clauses_l_init (already_propagated_unit_init_l C S) = add_mset C (get_unit_clauses_l_init S)\<close>
   \<open>get_learned_unit_clauses_l_init (already_propagated_unit_init_l C S) =
        get_learned_unit_clauses_l_init S\<close>
+  \<open>get_subsumed_learned_clauses_l_init (already_propagated_unit_init_l C S) =
+       get_subsumed_learned_clauses_l_init S\<close>
+  \<open>get_subsumed_init_clauses_l_init (already_propagated_unit_init_l C S) =
+       get_subsumed_init_clauses_l_init S\<close>
   \<open>get_conflict_l_init (T, OC) = get_conflict_l T\<close>
   by (solves \<open>cases S; cases T; auto simp: already_propagated_unit_init_l_def\<close>)+
 
@@ -764,8 +789,8 @@ proof -
     apply -
     apply normalize_goal+
     by presburger
-  obtain M N D NE UE Q U OC where
-    S: \<open>S = ((M, N, U, D, NE, UE, Q), OC)\<close>
+  obtain M N D NE UE Q U OC NS US where
+    S: \<open>S = ((M, N, U, D, NE, UE, NS, US, Q), OC)\<close>
     by (cases S) auto
   have [simp]: \<open>twl_list_invs (fst (already_propagated_unit_init_l (mset C) S))\<close>
     using add_inv by (auto simp:  already_propagated_unit_init_l_def S
@@ -797,10 +822,6 @@ proof -
     using dist WS dec in_literals_to_update OC'_empty nempty
     by (auto simp: twl_st_init twl_st_l_init)
 qed
-(*
-lemma (in -) uminus_list_of_mset_convert_lits_l:
-  \<open>{#- lit_of x. x \<in># mset (convert_lits_l N M)#} = {#- lit_of x. x \<in># mset M#}\<close>
-  by (induction M rule: ann_lit_list_induct)  auto *)
 
 lemma (in -) twl_stgy_invs_backtrack_lvl_0:
   \<open>count_decided (get_trail T) = 0 \<Longrightarrow> twl_stgy_invs T\<close>
@@ -835,8 +856,8 @@ proof -
     apply -
     apply normalize_goal+
     by presburger
-  obtain M N D NE UE Q U OC where
-    S: \<open>S = ((M, N, U, D, NE, UE, Q), OC)\<close>
+  obtain M N D NE UE Q U OC NS US where
+    S: \<open>S = ((M, N, U, D, NE, UE, NS, US, Q), OC)\<close>
     by (cases S) auto
   have 1: \<open>propagate_unit_init_l L S \<le> SPEC( \<lambda>S'. (S', propagate_unit_init L T)
         \<in> twl_st_l_init)\<close>
@@ -931,8 +952,8 @@ proof -
     apply -
     apply normalize_goal+
     by force
-  obtain M N D NE UE Q U OC where
-    S: \<open>S = ((M, N, U, D, NE, UE, Q), OC)\<close>
+  obtain M N D NE UE Q U OC NS US where
+    S: \<open>S = ((M, N, U, D, NE, UE, NS, US, Q), OC)\<close>
     by (cases S) auto
   have [simp]: \<open>twl_list_invs (fst (set_conflict_init_l C S))\<close>
     using add_inv by (auto simp:  set_conflict_init_l_def S
@@ -1006,14 +1027,14 @@ lemma twl_struct_invs_init_add_empty_conflict_init_l:
   shows \<open>twl_struct_invs_init (add_empty_conflict_init T)\<close>
       (is ?all_struct)
 proof -
-  obtain M N U D NE UE Q OC where
-    T: \<open>T = ((M, N, U, D, NE, UE, {#}, Q), OC)\<close>
+  obtain M N U D NE UE Q OC NS US where
+    T: \<open>T = ((M, N, U, D, NE, UE, NS, US, {#}, Q), OC)\<close>
     using WS by (cases T) auto
-  have \<open>cdcl\<^sub>W_restart_mset.cdcl\<^sub>W_all_struct_inv (M, clauses N + NE + OC, clauses U + UE, D)\<close>
+  have \<open>cdcl\<^sub>W_restart_mset.cdcl\<^sub>W_all_struct_inv (M, clauses N + NE + NS + OC, clauses U + UE + US, D)\<close>
     using invs unfolding T twl_struct_invs_init_def by auto
   then have [simp]:
-   \<open>cdcl\<^sub>W_restart_mset.cdcl\<^sub>W_all_struct_inv (M, add_mset {#} (clauses N + NE + OC),
-        clauses U + UE, Some {#})\<close>
+   \<open>cdcl\<^sub>W_restart_mset.cdcl\<^sub>W_all_struct_inv (M, add_mset {#} (clauses N + NE + NS + OC),
+        clauses U + UE + US, Some {#})\<close>
     unfolding T twl_struct_invs_init_def
     by (auto 5 5 simp: cdcl\<^sub>W_restart_mset.cdcl\<^sub>W_all_struct_inv_def
        cdcl\<^sub>W_restart_mset.no_strange_atm_def cdcl\<^sub>W_restart_mset_state
@@ -1022,24 +1043,24 @@ proof -
        clauses_def cdcl\<^sub>W_restart_mset.cdcl\<^sub>W_learned_clause_alt_def
        true_annots_true_cls_def_iff_negation_in_model)
 
-  have \<open>cdcl\<^sub>W_restart_mset.no_smaller_propa (M, clauses N + NE + OC, clauses U + UE, D)\<close>
+  have \<open>cdcl\<^sub>W_restart_mset.no_smaller_propa (M, clauses N + NE + NS + OC, clauses U + UE + US, D)\<close>
     using invs unfolding T twl_struct_invs_init_def by auto
   then have [simp]:
-     \<open>cdcl\<^sub>W_restart_mset.no_smaller_propa (M, add_mset {#} (clauses N + NE + OC),
-        clauses U + UE, Some {#})\<close>
+     \<open>cdcl\<^sub>W_restart_mset.no_smaller_propa (M, add_mset {#} (clauses N + NE + NS + OC),
+        clauses U + UE + US, Some {#})\<close>
     using lev
     by (auto simp: cdcl\<^sub>W_restart_mset.no_smaller_propa_def cdcl\<^sub>W_restart_mset_state
         clauses_def T count_decided_0_iff)
-  let ?T = \<open>(M, N, U, Some {#}, NE, UE, {#}, {#})\<close>
+  let ?T = \<open>(M, N, U, Some {#}, NE, UE, NS, US, {#}, {#})\<close>
 
   have [simp]: \<open>confl_cands_enqueued ?T\<close>
     \<open>propa_cands_enqueued ?T\<close>
-    \<open>twl_st_inv (M, N, U, D, NE, UE, {#}, Q) \<Longrightarrow> twl_st_inv ?T\<close>
-    \<open>\<And>x.  twl_exception_inv (M, N, U, D, NE, UE, {#}, Q) x \<Longrightarrow> twl_exception_inv ?T x\<close>
-    \<open>clauses_to_update_inv (M, N, U, D, NE, UE, {#}, Q) \<Longrightarrow> clauses_to_update_inv ?T\<close>
-    \<open>past_invs (M, N, U, D, NE, UE, {#}, Q) \<Longrightarrow> past_invs ?T\<close>
+    \<open>twl_st_inv (M, N, U, D, NE, UE, NS, US, {#}, Q) \<Longrightarrow> twl_st_inv ?T\<close>
+    \<open>\<And>x.  twl_exception_inv (M, N, U, D, NE, UE, NS, US, {#}, Q) x \<Longrightarrow> twl_exception_inv ?T x\<close>
+    \<open>clauses_to_update_inv (M, N, U, D, NE, UE, NS, US, {#}, Q) \<Longrightarrow> clauses_to_update_inv ?T\<close>
+    \<open>past_invs (M, N, U, D, NE, UE, NS, US, {#}, Q) \<Longrightarrow> past_invs ?T\<close>
     by (auto simp: twl_st_inv.simps twl_exception_inv.simps past_invs.simps; fail)+
-  have [simp]: \<open>entailed_clss_inv (M, N, U, D, NE, UE, {#}, Q) \<Longrightarrow> entailed_clss_inv ?T\<close>
+  have [simp]: \<open>entailed_clss_inv (M, N, U, D, NE, UE, NS, US, {#}, Q) \<Longrightarrow> entailed_clss_inv ?T\<close>
     using count_decided_ge_get_level[of M] lev by (auto simp: T)
   show ?all_struct
     using invs
@@ -1071,8 +1092,8 @@ proof -
     apply -
     apply normalize_goal+
     by force
-  obtain M N D NE UE Q U OC where
-    S: \<open>S = ((M, N, U, D, NE, UE, Q), OC)\<close>
+  obtain M N D NE UE Q U OC NS US where
+    S: \<open>S = ((M, N, U, D, NE, UE, NS, US, Q), OC)\<close>
     by (cases S) auto
   have [simp]: \<open>twl_list_invs (fst (add_empty_conflict_init_l S))\<close>
     using add_inv by (auto simp: add_empty_conflict_init_l_def S
@@ -1128,19 +1149,19 @@ lemma twl_struct_invs_init_add_to_clauses_init:
     \<open>twl_struct_invs_init (add_to_clauses_init C T)\<close>
       (is ?all_struct)
 proof -
-  obtain M N U NE UE OC WS where
-    T: \<open>T = ((M, N, U, None, NE, UE, WS, uminus `# lit_of `# mset M), OC)\<close>
+  obtain M N U NE UE OC WS NS US where
+    T: \<open>T = ((M, N, U, None, NE, UE, NS, US, WS, uminus `# lit_of `# mset M), OC)\<close>
     using confl MQ by (cases T) auto
   let ?Q = \<open>uminus `# lit_of `# mset M\<close>
   have [simp]: \<open>get_all_ann_decomposition M = [([], M)]\<close>
     by (rule no_decision_get_all_ann_decomposition) (use lev in \<open>auto simp: T count_decided_0_iff\<close>)
-  have \<open>cdcl\<^sub>W_restart_mset.cdcl\<^sub>W_all_struct_inv (M, (clauses N + NE + OC), clauses U + UE,  None)\<close> and
-    excep: \<open>twl_st_exception_inv (M, N, U, None, NE, UE, WS, ?Q)\<close> and
-    st_inv: \<open>twl_st_inv (M, N, U, None, NE, UE, WS, ?Q)\<close>
+  have \<open>cdcl\<^sub>W_restart_mset.cdcl\<^sub>W_all_struct_inv (M, (clauses N + NE + NS + OC), clauses U + UE + US,  None)\<close> and
+    excep: \<open>twl_st_exception_inv (M, N, U, None, NE, UE, NS, US, WS, ?Q)\<close> and
+    st_inv: \<open>twl_st_inv (M, N, U, None, NE, UE, NS, US, WS, ?Q)\<close>
     using invs confl unfolding T twl_struct_invs_init_def by auto
   then have [simp]:
-   \<open>cdcl\<^sub>W_restart_mset.cdcl\<^sub>W_all_struct_inv (M, add_mset (mset C) (clauses N + NE + OC),
-     clauses U + UE, None)\<close> and
+   \<open>cdcl\<^sub>W_restart_mset.cdcl\<^sub>W_all_struct_inv (M, add_mset (mset C) (clauses N + NE + NS + OC),
+     clauses U + UE + US, None)\<close> and
    n_d: \<open>no_dup M\<close>
     using dist_C
     by (auto simp: cdcl\<^sub>W_restart_mset.cdcl\<^sub>W_all_struct_inv_def
@@ -1148,21 +1169,21 @@ proof -
        cdcl\<^sub>W_restart_mset.cdcl\<^sub>W_M_level_inv_def cdcl\<^sub>W_restart_mset.cdcl\<^sub>W_conflicting_def
        cdcl\<^sub>W_restart_mset.distinct_cdcl\<^sub>W_state_def all_decomposition_implies_def
        clauses_def cdcl\<^sub>W_restart_mset.cdcl\<^sub>W_learned_clause_alt_def)
-  have \<open>cdcl\<^sub>W_restart_mset.no_smaller_propa (M, clauses N + NE + OC, clauses U + UE, None)\<close>
+  have \<open>cdcl\<^sub>W_restart_mset.no_smaller_propa (M, clauses N + NE + NS + OC, clauses U + UE + US, None)\<close>
     using invs confl unfolding T twl_struct_invs_init_def by auto
   then have [simp]:
-     \<open>cdcl\<^sub>W_restart_mset.no_smaller_propa (M, add_mset (mset C) (clauses N + NE + OC),
-        clauses U + UE,  None)\<close>
+     \<open>cdcl\<^sub>W_restart_mset.no_smaller_propa (M, add_mset (mset C) (clauses N + NE + NS + OC),
+        clauses U + UE + US,  None)\<close>
     using lev
     by (auto simp: cdcl\<^sub>W_restart_mset.no_smaller_propa_def cdcl\<^sub>W_restart_mset_state
         clauses_def T count_decided_0_iff)
 
-  let ?S = \<open>(M, N, U, None, NE, UE, WS, ?Q)\<close>
+  let ?S = \<open>(M, N, U, None, NE, UE, NS, US, WS, ?Q)\<close>
 
   have struct: \<open>struct_wf_twl_cls C\<close> if \<open>C \<in># N + U\<close> for C
     using st_inv that by (simp add: twl_st_inv.simps)
-  have \<open>entailed_clss_inv (fst T)\<close>
-    using invs unfolding T twl_struct_invs_init_def fst_conv by fast
+  have \<open>entailed_clss_inv (fst T)\<close> and subs: \<open>subsumed_clauses_inv (fst T)\<close>
+    using invs unfolding T twl_struct_invs_init_def fst_conv by fast+
   then have ent: \<open>entailed_clss_inv (fst (add_to_clauses_init C T))\<close>
     using lev by (auto simp: T get_level_cons_if)
   show \<open>twl_struct_invs_init (add_to_clauses_init C T)\<close>
@@ -1175,6 +1196,7 @@ proof -
     subgoal by (auto simp: T mset_take_mset_drop_mset')
     subgoal by (rule ent)
     subgoal by (auto simp: T)
+    subgoal using subs by (auto simp: T)
     done
 qed
 
@@ -1211,21 +1233,21 @@ proof -
     using SOC_T dec apply -
     apply (rule twl_st_l_init_no_decision_iff[THEN iffD2])
     using SOC_T dec SOC_T by (auto simp: twl_st_l_init twl_st_init convert_lits_l_def)
-  obtain M N NE UE Q OC where
-    S: \<open>S = ((M, N, None, NE, UE, {#}, Q), OC)\<close>
+  obtain M N NE UE Q OC NS US where
+    S: \<open>S = ((M, N, None, NE, UE, NS, US, {#}, Q), OC)\<close>
     using D WS by (cases S) auto
   have le_2: \<open>length a \<ge> 2\<close>
     using a by (cases a) auto
   have
-    \<open>init_dt_pre CS ((M, fmupd i (a, True) N, None, NE, UE, {#}, Q), OC)\<close> (is ?pre1) and
+    \<open>init_dt_pre CS ((M, fmupd i (a, True) N, None, NE, UE, NS, US, {#}, Q), OC)\<close> (is ?pre1) and
     \<open>init_dt_spec [a] S
-          ((M, fmupd i (a, True) N, None, NE, UE, {#}, Q), OC)\<close> (is ?spec1)
+          ((M, fmupd i (a, True) N, None, NE, UE, NS, US, {#}, Q), OC)\<close> (is ?spec1)
     if
       i_0: \<open>0 < i\<close> and
       i_dom: \<open>i \<notin># dom_m N\<close>
     for i :: \<open>nat\<close>
   proof -
-    let ?S = \<open>((M, fmupd i (a, True) N, None, NE, UE, {#}, Q), OC)\<close>
+    let ?S = \<open>((M, fmupd i (a, True) N, None, NE, UE, NS, US, {#}, Q), OC)\<close>
 (*     have [simp]: \<open>convert_lits_l (fmupd i (a, True) N) (NE+UE) convert_lits_l N (NE+UE)\<close>
       apply (rule convert_lits_l_cong)
       using add_inv i_dom i_0 by (auto simp: S twl_list_invs_def) *)
@@ -1256,7 +1278,7 @@ proof -
       subgoal by (use dec SOC_T in_literals_to_update dist in
           \<open>auto simp: S count_decided_0_iff twl_st_l_init twl_st_init le_2 inv\<close>)
       done
-    moreover have \<open>twl_list_invs (M, fmupd i (a, True) N, None, NE, UE, {#}, Q)\<close>
+    moreover have \<open>twl_list_invs (M, fmupd i (a, True) N, None, NE, UE, NS, US, {#}, Q)\<close>
       using add_inv i_dom i_0 by (auto simp: S twl_list_invs_def)
     moreover have \<open>twl_stgy_invs (fst (add_to_clauses_init a T))\<close>
       by (rule twl_stgy_invs_backtrack_lvl_0)
@@ -1301,10 +1323,10 @@ proof -
   have dec': \<open>\<forall>s\<in>set (get_trail_init T). \<not> is_decided s\<close>
     using SOC_T dec by (rule twl_st_l_init_no_decision_iff[THEN iffD2])
 
-  obtain M N D NE UE Q where
-    S: \<open>SOC = ((M, N, D, NE, UE, {#}, Q), OC)\<close>
+  obtain M N D NE UE NS US Q where
+    S: \<open>SOC = ((M, N, D, NE, UE, NS, US, {#}, Q), OC)\<close>
     using WS by (cases SOC) (auto simp: SOC)
-  then have S': \<open>S = (M, N, D, NE, UE, {#}, Q)\<close>
+  then have S': \<open>S = (M, N, D, NE, UE, NS, US, {#}, Q)\<close>
     using S unfolding SOC by auto
   show ?thesis
   proof (cases \<open>get_conflict_l (fst SOC)\<close>)
@@ -1322,17 +1344,17 @@ proof -
     then have [simp]: \<open>D = Some D'\<close>
       by (auto simp: S)
     have [simp]:
-       \<open>(((M, N, Some D', NE, UE, {#}, Q), add_mset (mset a) OC), add_to_other_init a T)
+       \<open>(((M, N, Some D', NE, UE, NS, US, {#}, Q), add_mset (mset a) OC), add_to_other_init a T)
          \<in> twl_st_l_init\<close>
       using SOC_T by (cases T; auto simp: S S' twl_st_l_init_def; fail)+
-    have \<open>init_dt_pre CS ((M, N, Some D', NE, UE, {#}, Q), add_mset (mset a) OC)\<close>
+    have \<open>init_dt_pre CS ((M, N, Some D', NE, UE, NS, US, {#}, Q), add_mset (mset a) OC)\<close>
       unfolding init_dt_pre_def
       apply (rule exI[of _ \<open>add_to_other_init a T\<close>])
       using dist inv WS dec' dec in_literals_to_update add_inv stgy_inv SOC_T
       by (auto simp: S' count_decided_0_iff twl_st_init
           intro!: twl_struct_invs_init_add_to_other_init)
-    moreover have \<open>init_dt_spec [a] ((M, N, Some D', NE, UE, {#}, Q), OC)
-        ((M, N, Some D', NE, UE, {#}, Q), add_mset (mset a) OC)\<close>
+    moreover have \<open>init_dt_spec [a] ((M, N, Some D', NE, UE, NS, US, {#}, Q), OC)
+        ((M, N, Some D', NE, UE, NS, US, {#}, Q), add_mset (mset a) OC)\<close>
       unfolding init_dt_spec_def
       apply (rule exI[of _ \<open>add_to_other_init a T\<close>])
       using dist inv WS dec dec' in_literals_to_update add_inv stgy_inv SOC_T
@@ -1479,7 +1501,7 @@ next
 qed
 
 lemma init_dt_pre_empty_state:
-  \<open>init_dt_pre [] (([], fmempty, None, {#}, {#}, {#}, {#}), {#})\<close>
+  \<open>init_dt_pre [] (([], fmempty, None, {#}, {#}, {#}, {#}, {#},{#}), {#})\<close>
   unfolding init_dt_pre_def
   by (auto simp: twl_st_l_init_def twl_struct_invs_init_def twl_st_inv.simps
       twl_struct_invs_def twl_st_inv.simps cdcl\<^sub>W_restart_mset.cdcl\<^sub>W_all_struct_inv_def
@@ -1493,9 +1515,9 @@ lemma init_dt_pre_empty_state:
       cdcl\<^sub>W_restart_mset.conflict_non_zero_unless_level_0_def)
 
 lemma twl_init_invs:
-  \<open>twl_struct_invs_init (([], {#}, {#}, None, {#}, {#}, {#}, {#}), {#})\<close>
-  \<open>twl_list_invs ([], fmempty, None, {#}, {#}, {#}, {#})\<close>
-  \<open>twl_stgy_invs ([], {#}, {#}, None, {#}, {#}, {#}, {#})\<close>
+  \<open>twl_struct_invs_init (([], {#}, {#}, None, {#}, {#}, {#}, {#}, {#},{#}), {#})\<close>
+  \<open>twl_list_invs ([], fmempty, None, {#}, {#}, {#}, {#}, {#},{#})\<close>
+  \<open>twl_stgy_invs ([], {#}, {#}, None, {#}, {#}, {#}, {#}, {#}, {#})\<close>
   by (auto simp: twl_struct_invs_init_def twl_st_inv.simps twl_list_invs_def twl_stgy_invs_def
       past_invs.simps
       twl_struct_invs_def twl_st_inv.simps cdcl\<^sub>W_restart_mset.cdcl\<^sub>W_all_struct_inv_def
